

Lambda terms practice — Solutions

In reductions below, we underline the *redex* — *reducible expression* — which is being contracted in each term.

$$\begin{aligned} SKK &= \underline{(\lambda xyz.xz(yz))KK} \\ &= \underline{(\lambda yz.Kz(yz))K} \\ &= (\lambda z.\underline{Kz(Kz)}) \\ &= \lambda z.z \\ &= I \end{aligned}$$

$$\begin{aligned} BI &= \underline{(\lambda xyz.x(yz))I} \\ &= (\lambda yz.\underline{I(yz)}) \\ &= \lambda yz.(yz) \\ &= \lambda yz.yz \\ &= 1 \end{aligned}$$

$$\begin{aligned} SII &= \underline{(\lambda xyz.xz(yz))II} \\ &= \underline{(\lambda yz.Iz(yz))I} \\ &= (\lambda z.\underline{Iz(Iz)}) \\ &= (\lambda z.z(\underline{Iz})) \\ &= \lambda z.zz \\ &= \omega \end{aligned}$$

$$\begin{aligned} BI &= \underline{(\lambda xyz.x(yz))CS} \\ &= \underline{(\lambda yz.C(yz))S} \\ &= \lambda z.C(Sz) \\ &= \lambda z.(\lambda xyz.xzy)(Sz) \\ &=_{\alpha} \lambda v.(\lambda xyz.xzy)(Sv) \\ &= \lambda v.(\lambda yz.Svzy) \\ &= \lambda vyz.\underline{Svzy} \\ &= \lambda vyz.vy(zy) \\ &=_{\alpha} \lambda xyz.xy(zy) \end{aligned}$$

$$\begin{aligned}
\mathbf{W}\mathbf{W}\mathbf{I} &= \underline{(\lambda xy.xyy)\mathbf{W}\mathbf{I}} \\
&= \underline{(\lambda y.\mathbf{W}yy)\mathbf{I}} \\
&= \mathbf{W}\mathbf{I}\mathbf{I} \\
&= \underline{(\lambda xy.xyy)\mathbf{I}\mathbf{I}} \\
&= \underline{(\lambda y.\mathbf{I}yy)\mathbf{I}} \\
&= \underline{\mathbf{I}\mathbf{I}\mathbf{I}} \\
&= \underline{\mathbf{I}\mathbf{I}} \\
&= \mathbf{I}
\end{aligned}$$

$$\begin{aligned}
\mathbf{W}\mathbf{I}\mathbf{W} &= \underline{(\lambda xy.xyy)\mathbf{I}\mathbf{W}} \\
&= \underline{(\lambda y.\mathbf{I}yy)\mathbf{W}} \\
&= \underline{\mathbf{I}\mathbf{W}\mathbf{W}} \\
&= \mathbf{W}\mathbf{W} \\
&= (\lambda xy.xyy)\mathbf{W} \\
&= \lambda y.\mathbf{W}yy \\
&= \lambda y.(\lambda x'y'.x'y'y')yy \\
&= \lambda y.yyy \\
&=_{\alpha} \lambda x.xxx
\end{aligned}$$

$$\begin{aligned}
\mathbf{W}\mathbf{W}\mathbf{W} &= \underline{(\lambda xy.xyy)\mathbf{W}\mathbf{W}} \\
&= \underline{(\lambda y.\mathbf{W}yy)\mathbf{W}} \\
&= \mathbf{W}\mathbf{W}\mathbf{W}
\end{aligned}$$

$$\begin{aligned}
(\lambda xy.y(xy))\omega(\lambda z.z\mathbf{I}) &= \underline{(\lambda xy.y(xy))\omega(\lambda z.z\mathbf{I})} \\
&= \underline{(\lambda y.y(\omega y))(\lambda z.z\mathbf{I})} \\
&= \underline{(\lambda z.z\mathbf{I})(\omega(\lambda z.z\mathbf{I}))} \\
&= (\omega(\lambda z.z\mathbf{I}))\mathbf{I} \\
&= \omega(\lambda z.z\mathbf{I})\mathbf{I} \\
&= \underline{(\lambda x.xxx)(\lambda z.z\mathbf{I})}\mathbf{I} \\
&= \underline{(\lambda z.z\mathbf{I})(\lambda z.z\mathbf{I})}\mathbf{I} \\
&= \underline{((\lambda z.z\mathbf{I})\mathbf{I})}\mathbf{I} \\
&= (\underline{\mathbf{I}\mathbf{I}})\mathbf{I} \\
&= \mathbf{I}\mathbf{I} \\
&= \mathbf{I}
\end{aligned}$$

$$\begin{aligned}
(\lambda v.v\mathbf{K})[M, N] &= \underline{(\lambda v.v\mathbf{K})[M, N]} \\
&= [M, N]\mathbf{K} \\
&= (\lambda z.zMN)\mathbf{K} \\
&= \mathbf{K}MN && (\text{since } z \notin M, N) \\
&= M
\end{aligned}$$

$$\begin{aligned}
(\lambda v.v\mathbf{c}_0)[M, N] &= \underline{(\lambda v.v\mathbf{c}_0)[M, N]} \\
&= [M, N]\mathbf{c}_0 \\
&= (\lambda z.zMN)\mathbf{c}_0 \\
&= \mathbf{c}_0MN && (\text{since } z \notin M, N) \\
&= \underline{(\lambda f.z.z)MN} \\
&= \underline{(\lambda z.z)N} \\
&= N
\end{aligned}$$

$$\begin{aligned}
\mathbf{c}_2\mathbf{K}xyz &= \underline{(\lambda fz.f(fz))\mathbf{K}xyz} \\
&= \underline{(\lambda z.\mathbf{K}(\mathbf{K}z))xyz} \\
&= \underline{\mathbf{K}(\mathbf{K}x)yz} \\
&= \underline{(\mathbf{K}x)z} \\
&= x
\end{aligned}$$

$$\begin{aligned}
S^+\mathbf{c}_2 &= \underline{(\lambda n.fz.f(nfz))\mathbf{c}_2} \\
&= \lambda fz.f(\mathbf{c}_2fz) \\
&= \lambda fz.f(\underline{(\lambda f'z'.f'(f'z'))fz}) \\
&= \lambda fz.f(\underline{(\lambda z'.f(fz'))z}) \\
&= \lambda fz.f(f(fz)) \\
&= \mathbf{c}_3
\end{aligned}$$

$$\begin{aligned}
c_+ c_2 c_3 &= \underline{(\lambda m n f z . m f (n f z))} c_2 c_3 \\
&= \underline{(\lambda n f z . c_2 f (n f z))} c_3 \\
&= (\lambda f z . c_2 f (c_3 f z)) \\
&= \lambda f z . c_2 f (\underline{(\lambda f' z' . f' (f' (f' z')))} f z) \\
&= \lambda f z . c_2 f (\underline{(\lambda z' . f (f (f z')))} z) \\
&= \lambda f z . c_2 f (f (f (f z))) \\
&= \lambda f z . \underline{(\lambda f' z' . f' (f' (f' z')))} f (f (f (f z))) \\
&= \lambda f z . \underline{(\lambda z' . f (f z'))} (f (f (f z))) \\
&= \lambda f z . f (f (f (f (f z)))) \\
&= c_5
\end{aligned}$$

$$\begin{aligned}
c_\times c_2 c_3 &= \underline{(\lambda m n f . m (n f))} c_2 c_3 \\
&= \underline{(\lambda n f . c_2 (n f))} c_3 \\
&= (\lambda f . c_2 (c_3 f)) \\
&= \lambda f . (\lambda f z . f (f z)) (c_3 f) \\
&=_{\alpha} \lambda f . \underline{(\lambda g z . g (g z))} (c_3 f) \\
&= \lambda f . (\lambda z . (c_3 f) ((c_3 f) z)) \\
&= \lambda f . \lambda z . c_3 f (c_3 f z) \\
&= \lambda f z . c_3 f (\underline{(\lambda f' z' . f' (f' (f' z')))} f z) \\
&= \lambda f z . c_3 f (\underline{(\lambda z' . f (f (f z')))} z) \\
&= \lambda f z . c_3 f (f (f (f z))) \\
&= \lambda f z . \underline{(\lambda f' z' . f' (f' (f' z')))} f (f (f (f z))) \\
&= \lambda f z . \underline{(\lambda z' . f (f (f z')))} (f (f (f z))) \\
&= \lambda f z . f (f (f (f (f z)))) \\
&= c_6
\end{aligned}$$

$$\begin{aligned}
c_1 \wedge c_2 c_3 &= (\lambda mn.nm)c_2 c_3 \\
&= (\lambda n.n c_2)c_3 \\
&= c_3 c_2 \\
&= (\lambda fz.f(f(fz)))c_2 \\
&= \lambda z.c_2(c_2(c_2z)) \\
&=_{\alpha} \lambda x.c_2(c_2(c_2x)) \\
&= \lambda x.(\lambda fz.f(fz))(c_2(c_2x)) \\
&= \lambda x.(\lambda z.(c_2(c_2x))((c_2(c_2x))z)) \\
&= \lambda x.\lambda z.(c_2(c_2x))(c_2(c_2x)z) \\
&= \lambda xz.c_2(c_2x)(c_2(c_2x)z) \\
&=_{\alpha} \lambda xy.c_2(c_2x)(c_2(c_2x)y) \\
&= \lambda xy.c_2(c_2x)((\lambda fz.f(fz))(c_2x)y) \\
&= \lambda xy.c_2(c_2x)((c_2x)((c_2x)y)) \\
&= \lambda xy.c_2(c_2x)(c_2x(c_2xy)) \\
&= \lambda xy.c_2(c_2x)(c_2x((\lambda fz.f(fz))xy)) \\
&= \lambda xy.c_2(c_2x)(c_2x(x(xy))) \\
&= \lambda xy.c_2(c_2x)((\lambda fz.f(fz))x(x(xy))) \\
&= \lambda xy.c_2(c_2x)((\lambda z.x(xz))(x(xy))) \\
&= \lambda xy.c_2(c_2x)(x(x(x(xy)))) \\
&= \lambda xy.c_2(c_2x)(x^4y) \\
&= \lambda xy.(\lambda fz.f(fz))(c_2x)(x^4y) \\
&= \lambda xy.((c_2x)((c_2x)(x^4y))) \\
&= \lambda xy.c_2x(c_2x(x^4y)) \\
&= \lambda xy.c_2x((\lambda fz.f(fz))x(x^4y)) \\
&= \lambda xy.c_2x(x(x(x^4y))) \\
&= \lambda xy.(\lambda fz.f(fz))x(x^6y) \\
&= \lambda xy.(x(x(x^6y))) \\
&= \lambda xy.x^8y \\
&= c_8
\end{aligned}$$

$$\begin{aligned}
c_4CK &= (\lambda fz.f(f(f(fz))))CK \\
&= C(C(C(CK))) \\
&= \underline{(\lambda xyz.xzy)(C(C(CK)))} \\
&= \lambda yz.(C(C(CK)))zy \\
&= \lambda yz.\underline{(\lambda x'y'z'.x'z'y')(C(CK))zy} \\
&= \lambda yz.(C(CK))yz \\
&= \lambda yz.\underline{(\lambda x'y'z'.x'z'y')(CK)yz} \\
&= \lambda yz.(CK)zy \\
&= \lambda yz.\underline{(\lambda x'y'z'.x'z'y')Kzy} \\
&= \lambda yz.\underline{Kyz} \\
&= \lambda yz.y \\
&= K
\end{aligned}$$